DFSSpec.v
@@ -13,7 +13,7 @@ Module Type DFSBase (O: UsualOrderedType)(S: FSetInterface.Sfun O)(G: Graph O S)
   
   Parameter dfs : option G.vertex -> G.graph -> (F.forest *  times_function * times_function).
 
-  Parameter state : G.graph -> Type.
+  Parameter state : option G.vertex -> G.graph -> Type.
 
   Definition d_time o g := match (dfs o g) with
                            | (_, f, _) => f
@@ -33,44 +33,44 @@ Module Type DFSBase (O: UsualOrderedType)(S: FSetInterface.Sfun O)(G: Graph O S)
 
   Parameter d_time : G.graph -> G.vertex -> nat.*)
 
-  Parameter time_of_state: forall g, state g -> nat. 
+  Parameter time_of_state: forall o g, state o g -> nat. 
 
   (* States must exist*)
   Parameter discovery_exists: forall o g v,
     G.contains_vertex g v = true ->
-    exists (s: state g), time_of_state g s = d_time o g v.
+    exists (s: state o g), time_of_state o g s = d_time o g v.
 
-  Parameter finish_exists: forall o g v,
+  (*Parameter finish_exists: forall o g v,
     G.contains_vertex g v = true ->
-    exists (s: state g), time_of_state g s = d_time o g v.
+    exists (s: state o g), time_of_state o g s = f_time o g v.*)
 
-  Definition white o g (s: state g)(v: G.vertex) : bool :=
-    ltb (time_of_state g s) (d_time o g v).
+  Definition white o g (s: state o g)(v: G.vertex) : bool :=
+    ltb (time_of_state o g s) (d_time o g v).
 
-  Definition gray o g (s: state g)(v: G.vertex): bool :=
-    ltb (time_of_state g s) (f_time o g v) && leb (d_time o g v) (time_of_state g s).
+  Definition gray o g (s: state o g)(v: G.vertex): bool :=
+    ltb (time_of_state o g s) (f_time o g v) && leb (d_time o g v) (time_of_state o g s).
 
-  Definition black o g (s:state g)(v: G.vertex) : bool :=
-    leb (f_time o g v) (time_of_state g s).
+  Definition black o g (s:state o g)(v: G.vertex) : bool :=
+    leb (f_time o g v) (time_of_state o g s).
 
-  Parameter state_time_unique: forall g (s s': state g),
-    time_of_state g s = time_of_state g s' <-> s = s'.
+  Parameter state_time_unique: forall g o (s s': state o g),
+    time_of_state o g s = time_of_state o g s' <-> s = s'.
 
   (* Some needed results about uniqueness of times *)
-  Parameter d_times_unique: forall o g u v
-    (Hu: G.contains_vertex g u = true)
-    (Hv: G.contains_vertex g v = true),
+  Parameter d_times_unique: forall o g u v,
+    G.contains_vertex g u = true ->
+    G.contains_vertex g v = true ->
     d_time o g u = d_time o g v <-> u = v.
 
-  Parameter f_times_unique: forall o g u v
-    (Hu: G.contains_vertex g u = true)
-    (Hv: G.contains_vertex g v = true),
+  Parameter f_times_unique: forall o g u v,
+    G.contains_vertex g u = true ->
+    G.contains_vertex g v = true ->
     f_time o g u = f_time o g v <-> u = v.
 
   Parameter all_times_unique:
-    forall o g u v
-    (Hu: G.contains_vertex g u = true)
-    (Hv: G.contains_vertex g v = true),
+    forall o g u v,
+    G.contains_vertex g u = true ->
+    G.contains_vertex g v = true ->
     f_time o g u <> d_time o g v.
 
   (*Major Results*)
@@ -91,7 +91,7 @@ Module Type DFSBase (O: UsualOrderedType)(S: FSetInterface.Sfun O)(G: Graph O S)
 
   Parameter white_path_theorem: forall o g u v,
     G.contains_vertex g u = true ->
-    F.desc (dfs_forest o g) u v <-> (forall s, time_of_state g s = d_time o g u ->
+    F.desc (dfs_forest o g) u v <-> (forall s, time_of_state o g s = d_time o g u ->
     exists l, P.path_list_ind g u v (fun x => white o g s x) l).
 
   (* Basic results about vertices and edges *)
@@ -109,87 +109,3 @@ Module Type DFSBase (O: UsualOrderedType)(S: FSetInterface.Sfun O)(G: Graph O S)
     d_time (Some v) g v < d_time (Some v) g u.
 
 End DFSBase.
-(*
-(*TODO: figure out how to not copy everything and fix types*)
-Module Type DFSWithStart (O: UsualOrderedType)(S: FSetInterface.Sfun O)(G: Graph O S)(F: Forest O S G).
-
-  Module P := (Path.PathTheories O S G).
-
-  Section WithGraph.
-
-  Variable (g: G.graph).
-  
-  Parameter dfs_start : G.vertex -> G.graph -> F.forest.
-
-  Parameter state : G.graph -> Type.
-
-  Parameter f_time : G.graph -> G.vertex -> nat.
-
-  Parameter d_time : G.graph -> G.vertex -> nat.
-
-  Notation "'d' x" := (d_time g x)(at level 40).
-  Notation "'f' x" :=(f_time g x)(at level 40).
-
-  Parameter time_of_state : state g -> nat.
-
-  Definition white (s: state g)(v: G.vertex) : bool :=
-    ltb (time_of_state s) (d v).
-
-  Definition gray (s: state g)(v: G.vertex): bool :=
-    ltb (time_of_state s) (f v) && leb (d v) (time_of_state s).
-
-  Definition black (s:state g)(v: G.vertex) : bool :=
-    leb (f v) (time_of_state s).
-
-  Parameter state_time_unique: forall (s s': state g),
-    time_of_state s = time_of_state s' <-> s = s'.
-
-Section ValidVertex.
-
-  Variable (u v: G.vertex).
-  Variable (Hu: G.contains_vertex g u = true).
-  Variable (Hv: G.contains_vertex g v = true).
-
-  (* Some needed results about uniqueness of times *)
-  Parameter d_times_unique: forall  u v,
-    d u = d v <-> u = v.
-
-  Parameter f_times_unique: forall u v,
-    f u = f v <-> u = v.
-
-  Parameter all_times_unique: forall u v,
-    f u <> d v.
-
-  (*Major Results*)
-  Parameter parentheses_theorem: 
-    u <> v ->
-    (d u < d v /\ d v < f v /\ f v < f u) \/ (d v < d u /\ d u < f u /\ f u < f v) \/
-    (d u < f u /\ f u < d v /\ d v < f v) \/ (d v < f v /\ f v < d u /\ d u < f u).
-
-  Parameter descendant_iff_interval: forall a, 
-    F.desc (dfs_start a g) u v <-> (d u < d v /\ d v < f v /\ f v < f u).
-
-  Parameter white_path_theorem: forall s a,
-    F.desc (dfs_start a g) u v <-> (time_of_state s = d u ->
-    exists l, P.path_list_ind g u v (fun x => white s x) l).
-
-End ValidVertex.
-End WithGraph.
-
-  (* Basic results about vertices and edges *)
-  Parameter same_vertices: forall g v a,
-    G.contains_vertex g v = true <-> F.contains_vertex (dfs_start a g) v = true.
-
-  Parameter same_edges: forall g u v a,
-    F.is_child (dfs_start a g) u v = true -> G.contains_edge g u v = true.
-
-  (*Why we care about starting from a specific vertex*)
-  Parameter start_vertex: forall g a u,
-    G.contains_vertex g a = true ->
-    G.contains_vertex g u = true ->
-    a <> u ->
-    d_time g a < d_time g u.
-End DFSWithStart.
-*)
-
-  
